ToSSA Continue & FromSSA

DuplicateStatement/DuplicateStatement.dfy
@@ -8,23 +8,85 @@ type BooleanExpression = string
 class VariablesSSA {
 
 	var m: map<Variable, seq<Variable>>;
+	var n: int;
+
+	constructor ()
+		modifies this
+		ensures n == 1
+	{
+		n := 1;
+	}
+
+	method getAndIncN() returns (res: int)
+		modifies this
+		requires n >= 1
+		ensures n >= 2
+		ensures res >= 1
+	{
+		res := n;
+		n := n + 1;
+	}
 
 	method variablesToSSAVariables(variables: seq<Variable>, instances: seq<Variable>)
+		requires |instances| == |variables|
+		modifies this
 	{
-		if !(variables == []) { addVariable(variables[0], instances[0]); variablesToSSAVariables(variables[1..], instances[1..]); }
+		if !(variables == [])
+		{
+			addVariable(variables[0], instances[0]);
+			variablesToSSAVariables(variables[1..], instances[1..]);
+		}
 	}
 
 	method addVariable(v: Variable, vSSA: Variable)
+		modifies this
 	{
 		if v in m { m := m[v := m[v] + [vSSA]]; } else { m := m[v := [vSSA]]; }
 	}
 
-	function method getVariableInRegularForm(vSSA: Variable)  : Variable
+	method getVariableInRegularForm(vSSA: Variable)  returns (v : Variable)
+		requires existsVSSA(vSSA)
 	{
-		var v :| v in m;
-		var values := m[v];
+		v :| v in m && vSSA in m[v]; 
+	}
 
-		if vSSA in values then v else getVariableInRegularForm(vSSA, m - v)
+	predicate existsVSSA(vSSA: Variable)
+		reads this
+	{
+		exists v :: v in m && vSSA in m[v]
+	}
+
+	method instancesToVariables(instances: seq<Variable>) returns (V : seq<Variable>)
+		requires forall i :: i in instances ==> existsVSSA(i)
+		ensures |instances| == |V|
+		
+	{
+		if instances == [] { V := []; } 
+		else { 
+			var v := getVariableInRegularForm(instances[0]);
+			var V' := instancesToVariables(instances[1..]);
+
+			V := [v] + V';
+		}
+	}
+
+	method getInstancesOfVarible(v : Variable) returns (instances : seq<Variable>)
+		requires v in m
+		requires |m[v]| >= 1
+		ensures |instances| >= 1
+	{
+		instances := m[v];
+	}
+
+	method getInstancesOfVaribleSeq(V : seq<Variable>) returns (instances : seq<Variable>)
+		requires forall v :: v in V ==> v in m && |m[v]| >= 1
+	{
+		if V == [] { instances := []; }
+		else {
+			var vInstaces := getInstancesOfVarible(V[0]);
+			var instances' := getInstancesOfVaribleSeq(V[1..]);
+			instances := vInstaces + instances';
+		}
 	}
 }
 
@@ -116,16 +178,73 @@ predicate method ValidAssignment(str : string)
 	true // check ":=" with same-length lists to its left and right, the former of distinct variable names and the right of expressions
 }
 
-
-function method freshInit(vars : seq<Variable>, ghost allVars : set<Variable>) : seq<Variable>
-	//requires |setOf(vars)| == |vars|;
-	requires setOf(vars) < allVars;
-	requires forall v :: v in vars ==> "i"+v !in allVars;
-	ensures setOf(freshInit(vars,allVars)) !! allVars;
-	ensures setOf(freshInit(vars,allVars)) !! allVars;
-	ensures |freshInit(vars,allVars)| == |vars|;
+predicate Valid(stmt: Statement) reads *
 {
-	if vars == [] then [] else ["i"+vars[0]] + freshInit(vars[1..],allVars+{"i"+vars[0]})
+	match stmt {
+		case Skip => true
+		case Assignment(LHS, RHS) => |LHS| == |RHS|
+		case SeqComp(S1,S2) => Valid(S1) && Valid(S2)
+		case IF(B,Sthen,Selse) => true
+			//(forall state: State :: B.requires(state) && B(state).Bool?) && 
+			//Valid(Sthen) && Valid(Selse)
+		case DO(B,S) => true
+			//(forall state: State :: B.requires(state) && B(state).Bool?) && Valid(S)
+		case LocalDeclaration(L,S) => Valid(S)
+	} 
+	//&&
+	//forall state1: State, P: Predicate  :: P.requires(state1)
+
+}
+
+method digitToString(num: int) returns (str: string)
+	requires num >= 0 && num <= 9
+{
+	if num == 0 { str := "0"; }
+	else if num == 1 { str := "1"; }
+	else if num == 2 { str := "2"; }
+	else if num == 3 { str := "3"; }
+	else if num == 4 { str := "4"; }
+	else if num == 5 { str := "5"; }
+	else if num == 6 { str := "6"; }
+	else if num == 7 { str := "7"; }
+	else if num == 8 { str := "8"; }
+	else if num == 9 { str := "9"; }
+}
+
+
+method intToString(num: int) returns (str: string)
+	requires num >= 0
+{
+	if num >= 0 && num <= 9 { str := digitToString(num); }
+	else
+	{
+		var digitStr := digitToString(num % 10);
+		var str' := intToString(num / 10);
+		str := str' + digitStr;
+	}
+}
+
+ method freshInit(vars : seq<Variable>, ghost allVars : set<Variable>, vsSSA : VariablesSSA) returns (res: seq<Variable>)
+	//requires |setOf(vars)| == |vars|;
+	//requires setOf(vars) < allVars;
+	//requires forall v :: v in vars ==> "i"+v !in allVars;
+	requires vsSSA != null
+	requires vsSSA.n >= 1
+	//ensures setOf(res) !! allVars;
+	ensures |res| == |vars|;
+	modifies vsSSA
+{
+	// if vars == [] then [] else ["i"+vars[0]] + freshInit(vars[1..],allVars+{"i"+vars[0]})
+
+	if vars == [] { res := []; } 
+	else
+	{
+		var n := vsSSA.getAndIncN();
+		var nStr := intToString(n);
+		var res' := freshInit(vars[1..], allVars + {vars[0] + nStr}, vsSSA);
+
+		res := [vars[0] + nStr] + res';
+	}
 }
 
 function method def(S : Statement) : set<Variable> // FIXME: make it return a set
@@ -382,67 +501,244 @@ method ComputeFISlice(S: Statement, V: set<Variable>) returns (SV: Statement)
 	SV := ComputeSlides(S, Vstar);
 }
 
- method ToSSA(S: Statement, X: seq<Variable>, liveOnEntryX: seq<Variable>, liveOnExitX: seq<Variable>, Y: set<Variable>, XLs: set<Variable>) returns(S': Statement)
+/*function method setToSeq(s : set<Variable>) : seq<Variable>
+	requires |s| >= 1
 {
-	var vsSSA := new VariablesSSA;
+	var v :| v in s;
+
+	if |s| == 1 then [v] else [v] + setToSeq(s - {v})
+}*/
+
+
+ method setToSeq(s : set<Variable>) returns (res: seq<Variable>)
+{
+	if s == {} { res := []; }
+	else
+	{
+		var v :| v in s;
+		var res' := setToSeq(s - {v});
+
+		res := [v] + res';
+	}
+}
+
+
+
+method ToSSA(S: Statement, X: seq<Variable>, liveOnEntryX: seq<Variable>, liveOnExitX: seq<Variable>, Y: set<Variable>, XLs: set<Variable>, vsSSA: VariablesSSA) returns(S': Statement)
+	requires Valid(S)
+	requires vsSSA != null
+{
+	//var vsSSA := new VariablesSSA(); // Create in main!
 
 	match S {
 		case Assignment(LHS,RHS) => S' := AssignmentToSSA(LHS, RHS, X, liveOnEntryX, liveOnExitX, Y, XLs, vsSSA);
 		case SeqComp(S1,S2) => S' := SeqCompToSSA(S1, S2, X, liveOnEntryX, liveOnExitX, Y, XLs, vsSSA);
 		case IF(B0,Sthen,Selse) => S' := IfToSSA(B0, Sthen, Selse, X, liveOnEntryX, liveOnExitX, Y, XLs, vsSSA);
 		case DO(B,S) => S' := DoToSSA(B, S, X, liveOnEntryX, liveOnExitX, Y, XLs, vsSSA);
+		case LocalDeclaration(L,S0) => S' := Skip;
+		case Skip => S' := Skip;
 	}
 }
 
-method AssignmentToSSA(LHS: seq<Variable>, RHS: seq<Variable>, X: seq<Variable>, liveOnEntryX: seq<Variable>, liveOnExitX: seq<Variable>, Y: set<Variable>, XLs: set<Variable>, vsSSA: VariablesSSA) returns (S': Statement)
+method IsVariableInSet(v: Variable, X: set<Variable>) returns (isInSet: bool)
 {
-	var copyLHS := setOf(LHS);
-	var X4 := copyLHS * setOf(liveOnEntryX) * setOf(liveOnExitX);
-	
-	copyLHS := copyLHS - X4;
-	var X5 := copyLHS * setOf(liveOnExitX);
-
-	copyLHS := copyLHS - X5;
-	var X2 := copyLHS * setOf(liveOnEntryX);
-
-	copyLHS := copyLHS - X2;
-	var Y1 := copyLHS * Y;
-
-	copyLHS := copyLHS - Y;
-	var X6 := copyLHS;
-
-	var XL4f := X4;
-	var XL5f := X5;
-
-	//var XL2XL6 := freshInit([X2, X6], setOf(X)+Y+XLs);
-
-	var X2X6Seq := setToSeq(X2) + setToSeq(X6);
-	var XL2XL6 := freshInit(X2X6Seq, setOf(X)+Y+XLs);
-		
-		vsSSA.variablesToSSAVariables(X2X6Seq, XL2XL6);
-
-	var LHS' := [XL4f, XL2XL6[..|X2|], XL5f, XL2XL6[|X2|..], Y1];
-	var RHS' := []; // TODO 
-
-	S' := Assignment(LHS', RHS') ;
+	if X == {} { isInSet := false; }
+	else
+	{
+		var x :| x in X;
+		if x == v { isInSet := true; }
+		else
+		{
+			 isInSet := IsVariableInSet(v, X - {x});
+		}
+	}
 }
 
-function method setToSeq(s : set<Variable>) : seq<Variable>
+method GetXandE(LHS: seq<Variable>, RHS: seq<Expression>, X: set<Variable>) returns (XSeq: seq<Variable>, ESeq: seq<Expression>)
+	requires Valid(Assignment(LHS,RHS))
 {
-	var v :| v in s;
+	if LHS == [] { XSeq:= []; ESeq := []; }
+	else
+	{
+		var x, e := [], [];
+		var isVariableInSet := IsVariableInSet(LHS[0], X);
+		
+		if isVariableInSet == true
+		{
+			x := [LHS[0]];
+			e := [RHS[0]];
+		}
 
-	if s == {} then [] else [v] + setToSeq(s - {v})
+		var XSeq', ESeq' := GetXandE(LHS[1..], RHS[1..], X);
+
+		XSeq := x + XSeq';
+		ESeq := e + ESeq';
+	}
+}
+
+method GetInstanceAccordingToX(x: Variable, instancesOfX: set<Variable>, vsSSA: VariablesSSA) returns (x': Variable)
+	requires vsSSA != null
+	requires |instancesOfX| >= 1
+	requires x in vsSSA.m
+{
+	var i :| i in instancesOfX;
+
+	if |instancesOfX| == 1 { x' := i; }
+	else if i in vsSSA.m[x] { x' := i; }
+	else
+	{
+		x' := GetInstanceAccordingToX(x, instancesOfX - {i}, vsSSA);
+	}
+}
+
+method InstancesSetToSeq(instancesOfX: set<Variable>, X: seq<Variable>, vsSSA: VariablesSSA) returns (instancesOfXSeq: seq<Variable>)
+	requires vsSSA != null
+	requires instancesOfX != {}
+	requires forall x :: x in X ==> x in vsSSA.m && |vsSSA.m[x]| >= 1
+{
+	// For example: instancesOfX	= {b2,a3,c1}
+	//				X				= [a,b,c]
+	//				instancesOfXSeq = [a3,b2,c1]	
+
+	if X == [] { instancesOfXSeq := []; }
+	else
+	{
+		var i := GetInstanceAccordingToX(X[0], instancesOfX, vsSSA);					// i = a3
+		var instancesOfXSeq' := InstancesSetToSeq(instancesOfX, X[1..], vsSSA);			// instancesOfXSeq = [b2,c1]
+		
+		instancesOfXSeq := [i] + instancesOfXSeq';										// instancesOfXSeq = [a3,b2,c1]
+	}
+}
+
+method SubstitueExpressionSeq(E: seq<Expression>, X: seq<set<Variable>>, XLi: seq<set<Variable>>) returns (E': seq<Expression>)
+{
+	// TODO - OR!
+}
+
+method SubstitueBooleanExpression(B: BooleanExpression, X: seq<set<Variable>>, XLi: seq<set<Variable>>) returns (B': BooleanExpression)
+{
+	// TODO - OR!
+}
+
+method AssignmentToSSA(LHS: seq<Variable>, RHS: seq<Expression>, X: seq<Variable>, liveOnEntryX: seq<Variable>, liveOnExitX: seq<Variable>, Y: set<Variable>, XLs: set<Variable>, vsSSA: VariablesSSA) returns (S': Statement)
+	requires vsSSA != null
+	requires Valid(Assignment(LHS,RHS))
+	
+{
+	// defined in thesis:
+	// toSSA.("X4,X2,X5,X6,Y1 := E1,E2,E3,E4,E5",
+	// X, (XL1i, XL2i, XL3i, XL4i), (XL3i, XL4f ,XL5f), Y ,XLs)) is:
+	// "XL4f, XL2, XL5f, XL6, Y1 := E1', E2', E3', E4', E5'"
+
+	//// find X1,X2,X3,X4,X5,X6,Y1 SETS ////
+
+	var XL3i := setOf(liveOnEntryX) * setOf(liveOnExitX);
+	var temp := setToSeq(XL3i);
+	var X3Seq := vsSSA.instancesToVariables(temp);
+	var X3 := setOf(X3Seq);
+
+	var XL1iXL2iXL4i := setOf(liveOnEntryX) - XL3i;
+	temp := setToSeq(XL1iXL2iXL4i);
+	var X1X2X4 := vsSSA.instancesToVariables(temp);
+	var XL4fXL5f := setOf(liveOnExitX) - XL3i;
+
+	temp := setToSeq(XL4fXL5f);
+	var X4X5 := vsSSA.instancesToVariables(temp);
+	var X4 := setOf(X1X2X4) * setOf(X4X5);
+	var X5 := setOf(X4X5) - X4;
+
+	var X1X2 := setOf(X1X2X4) - X4;
+	var X2 := X1X2 * def(Assignment(LHS,RHS));
+	var X1 := X1X2 - X2;
+
+	var X6Y1 := setOf(liveOnEntryX) - X4 - X2 - X5;
+	var X6 := setOf(X) * X6Y1;
+	var Y1 := X6Y1 - X6;
+
+	////////////////////////////////////////
+
+	var E1, E2, E3, E4, E5;
+	var X4Seq, X2Seq, X5Seq, X6Seq, Y1Seq;
+
+	X4Seq, E1 := GetXandE(LHS, RHS, X4);
+	X2Seq, E2 := GetXandE(LHS, RHS, X2);
+	X5Seq, E3 := GetXandE(LHS, RHS, X5);
+	X6Seq, E4 := GetXandE(LHS, RHS, X6);
+	Y1Seq, E5 := GetXandE(LHS, RHS, Y1);
+	
+	////////////////////////////////////////
+	//assert forall v :: v in X4Seq ==> v in vsSSA.m && |vsSSA.m[v]| >= 1;
+	var X4Instances := vsSSA.getInstancesOfVaribleSeq(X4Seq);
+	var XL5f := XL4fXL5f - setOf(X4Instances);
+	var XL4f := XL4fXL5f - XL5f;
+
+	var XL5fSeq := InstancesSetToSeq(XL5f, X5Seq, vsSSA);
+	var XL4fSeq := InstancesSetToSeq(XL4f, X4Seq, vsSSA);
+
+	////////////////////////////////////////
+
+	var E1', E2', E3', E4', E5';
+	var XL1iXL2i := XL1iXL2iXL4i - setOf(X4Instances);
+	var XL4i := XL1iXL2iXL4i - XL1iXL2i;
+
+	var X2Instances := vsSSA.getInstancesOfVaribleSeq(X2Seq);
+	var XL1i := XL1iXL2i - setOf(X2Instances);
+	var XL2i := XL1iXL2i - XL1i;
+
+	E1' := SubstitueExpressionSeq(E1, [X1,X2,X3,X4], [XL1i,XL2i,XL3i,XL4i]);
+	E2' := SubstitueExpressionSeq(E2, [X1,X2,X3,X4], [XL1i,XL2i,XL3i,XL4i]);
+	E3' := SubstitueExpressionSeq(E3, [X1,X2,X3,X4], [XL1i,XL2i,XL3i,XL4i]);
+	E4' := SubstitueExpressionSeq(E4, [X1,X2,X3,X4], [XL1i,XL2i,XL3i,XL4i]);
+	E5' := SubstitueExpressionSeq(E5, [X1,X2,X3,X4], [XL1i,XL2i,XL3i,XL4i]);
+
+	var XL2XL6 := freshInit(X2Seq + X6Seq, setOf(X)+Y+XLs, vsSSA);
+		 
+		vsSSA.variablesToSSAVariables(X2Seq + X6Seq, XL2XL6);
+
+	////////////////////////////////////////
+	
+	var LHS' := XL4fSeq + XL2XL6[..|X2|] + XL5fSeq + XL2XL6[|X2|..] + Y1Seq;
+	var RHS' := E1' + E2' + E3' + E4' + E5';
+
+	S' := Assignment(LHS', RHS');
 }
 
 method SeqCompToSSA(S1: Statement, S2: Statement, X: seq<Variable>, liveOnEntryX: seq<Variable>, liveOnExitX: seq<Variable>, Y: set<Variable>, XLs: set<Variable>, vsSSA: VariablesSSA) returns (S': Statement)
+	requires vsSSA != null
 {
-	var X3X4 := setOf(liveOnEntryX) * setOf(liveOnExitX);
-	var X4 := X3X4 * (def(S1) + def(S2));
-	var X3 := X3X4 - X4;
-	var X5 := setOf(liveOnExitX) - X3X4;
-	var X1X2 := setOf(liveOnEntryX) - X3X4;
-	var X2:= X1X2 * (def(S1) + def(S2));
+	// defined in thesis:
+	// toSSA.(" S1 ; S2 ", X, (XL1i, XL2i, XL3i, XL4i), (XL3i, XL4f, XL5f), Y, XLs) is:
+	// " S1' ; S2' "
+	
+	var XL3i := setOf(liveOnEntryX) * setOf(liveOnExitX);
+	var temp := setToSeq(XL3i);
+	var X3Seq := vsSSA.instancesToVariables(temp);
+	var X3 := setOf(X3Seq);
+
+	var liveOnEntryXVariables := vsSSA.instancesToVariables(liveOnEntryX);
+	var liveOnExitXVariables := vsSSA.instancesToVariables(liveOnExitX);
+	var X3X4 := setOf(liveOnEntryXVariables) * setOf(liveOnExitXVariables);
+	var X4 := X3X4 - X3;
+	var X5 := setOf(liveOnExitXVariables) - X3X4;
+
+	var X1X2 := setOf(liveOnEntryXVariables) - X3X4;
+	var X2 := X1X2 * (def(S1) + def(S2));
 	var X1 := X1X2 - X2;
+
+	var XL1iXL2iXL4i := setOf(liveOnEntryX) - XL3i;
+	temp := setToSeq(X4);
+	var X4Instances := vsSSA.getInstancesOfVaribleSeq(temp);
+	var XL1iXL2i := XL1iXL2iXL4i - setOf(X4Instances);
+	var XL4i := XL1iXL2iXL4i - XL1iXL2i;
+
+	temp := setToSeq(X2);
+	var X2Instances := vsSSA.getInstancesOfVaribleSeq(temp);
+	var XL1i := XL1iXL2i - setOf(X2Instances);
+	var XL2i := XL1iXL2i - XL1i;
+
+	var XL4fXL5f := setOf(liveOnExitX) - XL3i;
+	var XL5f := XL4fXL5f - setOf(X4Instances);
+	var XL4f := XL4fXL5f - XL5f;
 
 	var X6 := (setOf(X) - X3) * (((X4 + X5) - ddef(S2)) + input(S2)); 
 	var X11 := X1 * X6; 
@@ -452,60 +748,384 @@ method SeqCompToSSA(S1: Statement, S2: Statement, X: seq<Variable>, liveOnEntryX
 	var X51 := (X5 * X6) - def(S2);
 	var X61 := X6 - (X11+X21+X41+X42+X51); 
 
-	//var XL61 := freshInit(X61, setOf(X) + Y + XLs); // seq  // TODO 
 	var X61Seq := setToSeq(X61);
-	var XL61 := freshInit(X61Seq, setOf(X) + Y + XLs);
+	var XL61Seq := freshInit(X61Seq, setOf(X) + Y + XLs, vsSSA);
 		
-		vsSSA.variablesToSSAVariables(X61Seq, XL61);
+		vsSSA.variablesToSSAVariables(X61Seq, XL61Seq);
 
-	var XL6 := []; // TODO 
+	temp := setToSeq(X1);
+	var XL11iTemp := vsSSA.getInstancesOfVaribleSeq(temp);
+	var XL11iSeq := setToSeq(setOf(XL11iTemp) * XL1i);
+	temp := setToSeq(X2);
+	var XL21iTemp := vsSSA.getInstancesOfVaribleSeq(temp);
+	var XL21iSeq := setToSeq(setOf(XL21iTemp) * XL2i);
+	temp := setToSeq(X4);
+	var XL41iTemp := vsSSA.getInstancesOfVaribleSeq(temp);
+	var XL41iSeq := setToSeq(setOf(XL11iTemp) * XL4i);
+	temp := setToSeq(X4);
+	var XL42fTemp := vsSSA.getInstancesOfVaribleSeq(temp);
+	var XL42fSeq := setToSeq(setOf(XL11iTemp) * XL4f);
+	temp := setToSeq(X5);
+	var XL51fTemp := vsSSA.getInstancesOfVaribleSeq(temp);
+	var XL51fSeq := setToSeq(setOf(XL11iTemp) * XL5f);
+	temp := setToSeq(XL3i);
+	var XL6 := XL11iSeq + XL21iSeq + temp + XL41iSeq + XL42fSeq + XL51fSeq + XL61Seq;
 
-	var XLs' := XLs + setOf(XL61);
-	var S1' := ToSSA(S1, X, liveOnEntryX, XL6, Y, XLs');
+	var XLs' := XLs + setOf(XL61Seq);
+	var S1' := ToSSA(S1, X, liveOnEntryX, XL6, Y, XLs', vsSSA);
 	var XLs'' := XLs' + (glob(S1') - Y);
-	var S2' := ToSSA(S2, X, XL6, liveOnExitX, Y, XLs'');
+	var S2' := ToSSA(S2, X, XL6, liveOnExitX, Y, XLs'', vsSSA);
 
 	S' := SeqComp(S1', S2');
 }
 
-method IfToSSA(B : BooleanExpression, S1 : Statement, S2 : Statement, X: seq<Variable>, liveOnEntryX: seq<Variable>, liveOnExitX: seq<Variable>, Y: set<Variable>, XLs: set<Variable>, vsSSA: VariablesSSA) returns (S': Statement)
+method FindVariableIndexInVariableSequence(v: Variable, V: seq<Variable>) returns (i: int)
+	requires |V| >= 1
+	ensures i >= 0 && i < |V|
 {
-	var X4 := {};
-	var X5 := {};
+	if |V| == 1 { i := 0; }
+	else if V[0] == v { i := 0; }
+	else
+	{
+		i := FindVariableIndexInVariableSequence(v, V[1..]);
+		i := i + 1;
+	}
+}
 
-	var B' := B; // TODO
+method OrganizeVariables(vars1: seq<Variable>, vars2: seq<Variable>, vsSSA: VariablesSSA) returns (res: seq<Variable>)
+	requires vsSSA != null
+	requires forall i :: i in vars1 ==> vsSSA.existsVSSA(i)
+	requires forall i :: i in vars2 ==> vsSSA.existsVSSA(i)
+	requires |vars1| >= 0 && |vars2| >= 1
+{
+	if vars1 == [] { res := []; }
+	else
+	{
+		var v1 := vsSSA.getVariableInRegularForm(vars1[0]);
+		var vars2Variables := vsSSA.instancesToVariables(vars2);
+		var index := FindVariableIndexInVariableSequence(v1, vars2Variables);
+		var res' := OrganizeVariables(vars1[1..], vars2, vsSSA);
+
+		assert index < |vars2| && index >= 0;
+		res := [vars2[index]] + res';
+	}
+}
+
+method IfToSSA(B : BooleanExpression, S1 : Statement, S2 : Statement, X: seq<Variable>, liveOnEntryX: seq<Variable>, liveOnExitX: seq<Variable>, Y: set<Variable>, XLs: set<Variable>, vsSSA: VariablesSSA) returns (S': Statement)
+	requires vsSSA != null
+{
+	// defined in thesis:
+	// toSSA.(IF ,X, (XL1i, XL2i, XL3i, XL4i), (XL3i, XL4f, XL5f), Y, XLs) is:
+	// IF' where:
+	// IF := " if B then S1 else S2 fi "
+	// IF' := " if B' then S1'; XL4f ,XL5f := XL4t, XL5t else S2'; XL4f ,XL5f := XL4e, XL5e fi "
+
+	var XL3i := setOf(liveOnEntryX) * setOf(liveOnExitX);
+	var temp := setToSeq(XL3i);
+	var X3Seq := vsSSA.instancesToVariables(temp);
+	var X3 := setOf(X3Seq);
+
+	var XL4fXL5f := setOf(liveOnExitX) - XL3i;
+	temp := setToSeq(XL4fXL5f);
+	var X4X5 := vsSSA.instancesToVariables(temp);
+	var liveOnEntryXVariables := vsSSA.instancesToVariables(liveOnEntryX);
+	var X4 := setOf(liveOnEntryXVariables) * setOf(X4X5);
+	var X5Seq := setToSeq(setOf(X4X5) - X4);
+
+	var X2 := (setOf(liveOnEntryXVariables) - X4) * (def(S1) + def(S2));
+	var X1 := setOf(liveOnEntryXVariables) - X4 - X3 - X2;
+
+	var XL1iXL2iXL4i := setOf(liveOnEntryX) - XL3i;
+	temp := setToSeq(X4);
+	var X4Instances := vsSSA.getInstancesOfVaribleSeq(temp);
+	var XL1iXL2i := XL1iXL2iXL4i - setOf(X4Instances);
+	var XL4i := XL1iXL2iXL4i - XL1iXL2i;
+
+	temp := setToSeq(X2);
+	var X2Instances := vsSSA.getInstancesOfVaribleSeq(temp);
+	var XL1i := XL1iXL2i - setOf(X2Instances);
+	var XL2i := XL1iXL2i - XL1i;
+
+	var B' := SubstitueBooleanExpression(B, [X1,X2,X3,X4], [XL1i,XL2i,XL3i,XL4i]);
 	
-	var X4d1 := X4 * (def(S1) - def(S2)); // set
-	var X4d2 := X4 * (def(S2) - def(S1)); // set
-	var X4d1d2 := X4 * def(S1) * def(S2); // set
-	var freshRes := freshInit([X4d1, X4d2, X4d1d2, X4d1d2, X5, X5], setOf(X) + Y + XLs); // seq
+	var X4d1 := X4 * (def(S1) - def(S2));
+	var X4d2 := X4 * (def(S2) - def(S1));
+	var X4d1d2 := X4 * def(S1) * def(S2);
 
-	var XL4t := []; // TODO 
-	var XL4e := []; // TODO 
-	var XLs' := {}; // TODO 
+	temp := setToSeq(X4d1);
+	var temp1 := setToSeq(X4d2);
+	var temp2 := setToSeq(X4d1d2);
+	var temp3 := setToSeq(X4d1d2);
+	var variables := temp + temp1 + temp2 + temp3 + X5Seq + X5Seq;
+	var instances := freshInit(variables, setOf(X) + Y + XLs, vsSSA);
 
-	var S1' := ToSSA(S1, X, liveOnEntryX, [liveOnExitX[0], XL4t, freshRes[4]], Y, XLs');
+		vsSSA.variablesToSSAVariables(variables, instances);
+
+	var XL4d1t := instances[0..|X4d1|];
+	temp := setToSeq(X4d2);
+	var XL4d2iTemp := vsSSA.getInstancesOfVaribleSeq(temp);
+	var XL4d2iSeq := setToSeq(setOf(XL4d2iTemp) * XL4i);
+	var XL4d1d2t := instances[|X4d1|+|X4d2|..|X4d1|+|X4d2|+|X4d1d2|];
+	var XL4t := XL4d1t + XL4d2iSeq + XL4d1d2t;
+
+	temp := setToSeq(X4d1);
+	var XL4d1iTemp := vsSSA.getInstancesOfVaribleSeq(temp);
+	var XL4d1iSeq := setToSeq(setOf(XL4d1iTemp) * XL4i);
+	var XL4d2e := instances[|X4d1|..|X4d2|];
+	var XL4d1d1e := instances[|X4d1|+|X4d2|+|X4d1d2|..|X4d1|+|X4d2|+|X4d1d2|+|X4d1d2|];
+	var XL4e := XL4d1iSeq + XL4d2e + XL4d1d1e;
+
+	var XL5t := instances[|instances|-|X5Seq|-|X5Seq|..|instances|-|X5Seq|];
+	var XL5e := instances[|instances|-|X5Seq|..|instances|];
+
+	var XL5f := XL4fXL5f - setOf(X4Instances);
+	temp := setToSeq(XL5f);
+	var XL5fSeq := OrganizeVariables(XL5t, temp, vsSSA);
+	var XL4f := XL4fXL5f - XL5f;
+	temp := setToSeq(XL4f);
+	var XL4fSeqThen := OrganizeVariables(XL4t, temp, vsSSA);
+	temp := setToSeq(XL4f);
+	var XL4fSeqElse := OrganizeVariables(XL4e, temp, vsSSA);
+
+	var XLs' := XLs + setOf(instances);
+	temp := setToSeq(XL3i);
+	var S1' := ToSSA(S1, X, liveOnEntryX, (temp + XL4t + XL5t), Y, XLs', vsSSA);
 	var XLs'' := XLs' + (glob(S1') - Y);
-	var S2' := ToSSA(S2, X, liveOnEntryX, [liveOnExitX[0], XL4e, freshRes[5]], Y, XLs'');
-	
+	temp := setToSeq(XL3i);
+	var S2' := ToSSA(S2, X, liveOnEntryX, (temp + XL4e + XL5e), Y, XLs'', vsSSA);
 
-	S' := IF(B', SeqComp(S1', Assignment([X4, X5], [XL4t, freshRes[4]])), SeqComp(S2', Assignment([X4, X5], [XL4e, freshRes[5]])));
+	S' := IF(B', SeqComp(S1', Assignment(XL4fSeqThen + XL5fSeq, XL4t + XL5t)), SeqComp(S2', Assignment(XL4fSeqElse + XL5fSeq, XL4e + XL5e)));
 }
 
 method DoToSSA(B : BooleanExpression, S : Statement, X: seq<Variable>, liveOnEntryX: seq<Variable>, liveOnExitX: seq<Variable>, Y: set<Variable>, XLs: set<Variable>, vsSSA: VariablesSSA) returns (S'': Statement)
+	requires vsSSA != null
 {
-	var X4 := {};
-	var X3 := {};
-	var X2 := {};
-	var X1 := {};
+	// defined in thesis:
+	// toSSA.(DO, X, (XL1i, XL2i, XL3i, XL4i), (XL3i, XL4f), Y ,XLs) is:
+	// "XL2, XL4f := XL2i, XL4i; DO'" where:
+	// DO := " while B do S1 od ",
+	// DO' := " while B' do S1'; XL2, XL4f := XL2b, XL4b od "
 
-	var freshRes := freshInit([X2, X2, X4], setOf(X) + Y + XLs);
-	var XLs' := XLs + setOf([freshRes[0],freshRes[1],freshRes[2]]);
+	var XL4f := setOf(liveOnExitX) - (setOf(liveOnEntryX) * setOf(liveOnExitX));
+	var XL4fSeq := setToSeq(XL4f);
+	var temp := setToSeq(XL4f);
+	var X4Seq := vsSSA.instancesToVariables(temp);
+	var X4 := setOf(X4Seq);
 
-	var B' := B; // TODO 
+	var liveOnEntryXVariables := vsSSA.instancesToVariables(liveOnEntryX);
+	var X2 := (setOf(liveOnEntryXVariables) - X4) * def(S);
+	var X2Seq := setToSeq(X2);
+
+	var XL3i := setOf(liveOnEntryX) * setOf(liveOnExitX);
+	var XL3iSeq := setToSeq(XL3i);
+	var X3Seq := vsSSA.instancesToVariables(XL3iSeq);
+	var X3 := setOf(X3Seq);
 	
-	var S' := ToSSA(S, X, [X1, freshRes[0], X3, liveOnExitX[1]], [X1, freshRes[1], X3, freshRes[2]], Y, XLs');
-	var DO' := SeqComp(DO(B', S'), Assignment([freshRes[0], X4], [freshRes[1], freshRes[2]]));
+	var X1 := setOf(liveOnEntryXVariables) - X4 - X3 - X2;
 
-	S'' := SeqComp(Assignment([freshRes[0], X4], [X2, X4]), DO');
+	var variables := X2Seq + X2Seq + X4Seq;
+	var instances := freshInit(variables, setOf(X) + Y + XLs, vsSSA);
+
+		vsSSA.variablesToSSAVariables(variables, instances);
+
+	var XL2Seq := instances[0..|X2|];
+	var XL2bSeq := instances[|X2|..|X2|+|X2|];
+	var XL4bSeq := instances[|X2|+|X2|..];
+
+	var XL1iXL2iXL4i := setOf(liveOnEntryX) - (setOf(liveOnEntryX) * setOf(liveOnExitX));
+	var X4Instances := vsSSA.getInstancesOfVaribleSeq(X4Seq);
+	var XL1iXL2i := XL1iXL2iXL4i - setOf(X4Instances);
+	var XL4i := XL1iXL2iXL4i - XL1iXL2i;
+	temp := setToSeq(XL4i);
+	var XL4iSeq := OrganizeVariables(XL4fSeq, temp, vsSSA);
+
+	var X2Instances := vsSSA.getInstancesOfVaribleSeq(X2Seq);
+	var XL1i := XL1iXL2i - setOf(X2Instances);
+	var XL2i := XL1iXL2i - XL1i;
+	temp := setToSeq(XL2i);
+	var XL2iSeq := OrganizeVariables(XL2Seq, temp, vsSSA);
+	
+	////////////////////////////////////////
+
+	var XLs' := XLs + setOf(instances);
+	var B' := SubstitueBooleanExpression(B, [X1,X2,X3,X4], [XL1i,setOf(XL2Seq),XL3i,XL4f]);
+	temp := setToSeq(XL1i);
+	var temp1 := setToSeq(XL1i);
+	var S' := ToSSA(S, X, (temp + XL2Seq + XL3iSeq + XL4fSeq), (temp1 + XL2bSeq + XL3iSeq + XL4bSeq), Y, XLs', vsSSA);
+	var DO' := SeqComp(DO(B', S'), Assignment(XL2Seq + XL4fSeq, XL2bSeq + XL4bSeq));
+
+	S'' := SeqComp(Assignment(XL2Seq + XL4fSeq, XL2iSeq + XL4iSeq), DO');
+}
+
+
+
+
+
+method FromSSA(S': Statement, X: seq<Variable>, XL1i: seq<Variable>, XL2f: seq<Variable>, Y: set<Variable>, XLs: set<Variable>, vsSSA: VariablesSSA) returns( S: Statement)
+	decreases *
+	requires vsSSA != null
+	requires Valid(S')
+{
+	//var vsSSA := new VariablesSSA();
+
+	S := MergeVars(S', XLs, X, XL1i, XL2f, Y, vsSSA);
+}
+
+method MergeVars(S': Statement, XLs: set<Variable>, X: seq<Variable>, XL1i: seq<Variable>, XL2f: seq<Variable>, Y: set<Variable>, vsSSA: VariablesSSA) returns( S: Statement)
+	decreases *
+	requires vsSSA != null
+	requires Valid(S')
+{
+	match S' {
+		case Assignment(LHS,RHS) => S := AssignmentFromSSA(LHS, RHS, XLs, X, XL1i, XL2f, Y, vsSSA);
+		case SeqComp(S1',S2') => S := SeqCompFromSSA(S1', S2', XLs, X, XL1i, XL2f, Y, vsSSA);
+		case IF(B0,Sthen,Selse) => S := IfFromSSA(B0, Sthen, Selse, XLs, X, XL1i, XL2f, Y, vsSSA);
+		case DO(B,S') => S := DoFromSSA(B, S', XLs, X, XL1i, XL2f, Y, vsSSA);
+		case LocalDeclaration(L,S0) => S := Skip;
+		case Skip => S := Skip;
+	}
+}
+
+method AssignmentFromSSA(LHS: seq<Variable>, RHS: seq<Expression>, XLs: set<Variable>, X: seq<Variable>, XLi: seq<Variable>, XLf: seq<Variable>, Y: set<Variable>, vsSSA: VariablesSSA) returns (S: Statement)
+	requires vsSSA != null
+	requires Valid(Assignment(LHS,RHS))
+{
+	// defined in thesis:
+	// merge-vars.(" XL1f,XL2,XL3f,XL4,XL5f,XL6,Y1 := XL1i,XL2i,E1',E2',E3',E4',E5' ",
+	// XLs, X, (XL1i, XL2i, XL3i, XL4i, XL7i, XL8i), (XL1f, XL3f, XL5f, XL7i), Y) is:
+	// " X3,X4,X5,X6,Y1 := E1,E2,E3,E4,E5 "
+	
+	var Y1 := Y * def(Assignment(LHS, RHS)); // Y1 חיתוך בין Y ל def
+	var Y1Seq, E5' := GetXandE(LHS, RHS, Y1);
+
+	var XL7i := setOf(XLi) * setOf(XLf);
+	var temp := setToSeq(XL7i);
+	var X7Seq := vsSSA.instancesToVariables(temp);
+	var X7 := setOf(X7Seq);
+
+	var XL1iXL2i := setOf(XLi) * setOf(RHS);
+	temp := setToSeq(XL1iXL2i);
+	var X1X2 := vsSSA.instancesToVariables(temp);
+	var XL3iXL4iXL8i := setOf(XLi) - XL1iXL2i - XL7i;
+	temp := setToSeq(XL3iXL4iXL8i);
+	var X3X4X8 := vsSSA.instancesToVariables(temp);
+	var XL1fXL3fXL5f := setOf(XLf) - XL7i;
+	temp := setToSeq(XL1fXL3fXL5f);
+	var X1X3X5 := vsSSA.instancesToVariables(temp);
+
+	var X3 := setOf(X1X3X5) * setOf(X3X4X8);
+	temp := setToSeq(X3);
+	var X3Instances := vsSSA.getInstancesOfVaribleSeq(temp);
+	var XL3fSeq, E1' := GetXandE(LHS, RHS, setOf(X3Instances));
+
+	var XL1fXL5f := XL1fXL3fXL5f - setOf(XL3fSeq);
+	temp := setToSeq(XL1fXL5f);
+	var X1X5 := vsSSA.instancesToVariables(temp);
+	var X1 := setOf(X1X2) * setOf(X1X5);
+	temp := setToSeq(X1);
+	var X1Instances := vsSSA.getInstancesOfVaribleSeq(temp);
+	var XL1i := setOf(RHS) * setOf(X1Instances);
+	var XL1f := setOf(LHS) * setOf(X1Instances);
+	var XL5f := XL1fXL5f - XL1f;
+	var XL5fSeq, E3' := GetXandE(LHS, RHS, XL5f);
+	var X5SeqTemp := vsSSA.instancesToVariables(XL5fSeq);
+	var X5 := setOf(X5SeqTemp);
+
+	var XL2XL4XL6 := setOf(LHS) - XL1f - setOf(XL3fSeq) - XL5f - Y1;
+	var XL2i := XL1iXL2i - XL1i;
+	var X2 := setOf(X1X2) - X1;
+	temp := setToSeq(X2);
+	var X2Instances := vsSSA.getInstancesOfVaribleSeq(temp);
+	var XL2 := setOf(RHS) * setOf(X2Instances);
+	var XL4XL6 := XL2XL4XL6 - XL2;
+	temp := setToSeq(XL4XL6);
+	var X4X6 := vsSSA.instancesToVariables(temp);
+	var X4 := setOf(X3X4X8) * setOf(X4X6);
+	var X6 := setOf(X4X6) - X4;
+	temp := setToSeq(X4);
+	var X4Instances := vsSSA.getInstancesOfVaribleSeq(temp);
+	var XL4 := setOf(X4Instances) * setOf(LHS);
+	var XL6 := XL4XL6 - XL4;
+	var XL4Seq, E2' := GetXandE(LHS, RHS, XL4);
+	var XL6Seq, E4' := GetXandE(LHS, RHS, XL6);
+
+	var X8 := setOf(X3X4X8) - X3 - X4;
+	var XL3i := setOf(X3Instances) * setOf(XLi);
+	var XL4i := setOf(X4Instances) * setOf(XLi);
+	var XL8i := XL3iXL4iXL8i - XL3i - XL4i;
+
+	////////////////////////////////////////
+
+	var X3Seq := InstancesSetToSeq(X3, XL3fSeq, vsSSA);
+	var X4Seq := InstancesSetToSeq(X4, XL4Seq, vsSSA);
+	var X5Seq := InstancesSetToSeq(X5, XL5fSeq, vsSSA);
+	var X6Seq := InstancesSetToSeq(X6, XL6Seq, vsSSA);
+
+	////////////////////////////////////////
+
+	var E1, E2, E3, E4, E5;
+
+	E1 := SubstitueExpressionSeq(E1', [XL1i, XL2i, XL3i, XL4i, XL7i, XL8i], [X1, X2, X3, X4, X7, X8]);
+	E2 := SubstitueExpressionSeq(E2', [XL1i, XL2i, XL3i, XL4i, XL7i, XL8i], [X1, X2, X3, X4, X7, X8]);
+	E3 := SubstitueExpressionSeq(E3', [XL1i, XL2i, XL3i, XL4i, XL7i, XL8i], [X1, X2, X3, X4, X7, X8]);
+	E4 := SubstitueExpressionSeq(E4', [XL1i, XL2i, XL3i, XL4i, XL7i, XL8i], [X1, X2, X3, X4, X7, X8]);
+	E5 := SubstitueExpressionSeq(E5', [XL1i, XL2i, XL3i, XL4i, XL7i, XL8i], [X1, X2, X3, X4, X7, X8]);
+
+	S := Assignment(X3Seq + X4Seq + X5Seq + X6Seq + Y1Seq, E1 + E2 + E3 + E4 + E5);
+	//S := Skip;
+}
+
+method SeqCompFromSSA(S1': Statement, S2': Statement, XLs: set<Variable>, X: seq<Variable>, XLi: seq<Variable>, XLf: seq<Variable>, Y: set<Variable>, vsSSA: VariablesSSA) returns (S: Statement)
+	requires vsSSA != null
+	decreases *
+	requires Valid(SeqComp(S1',S2'))
+{
+	// defined in thesis:
+	// merge-vars.(" S1' ; S2' ", XLs, X, XL1i, XL2f, Y) is:
+	// " merge-vars.(S1', XLs, X, XL1i, XL3, Y) ; merge-vars.(S2', XLs, X, XL3, XL2f, Y) "
+
+	var XL3 := XLs * ((setOf(XLf) - ddef(S2')) + input(S2'));
+	var XL3Seq := setToSeq(XL3);
+
+	var S1 := MergeVars(S1', XLs, X, XLi, XL3Seq, Y, vsSSA);
+	var S2 := MergeVars(S2', XLs, X, XL3Seq, XLf, Y, vsSSA);
+
+	S := SeqComp(S1, S2);
+}
+
+method IfFromSSA(B' : BooleanExpression, S1' : Statement, S2' : Statement, XLs: set<Variable>, X: seq<Variable>, XLi: seq<Variable>, XLf: seq<Variable>, Y: set<Variable>, vsSSA: VariablesSSA) returns (S: Statement)
+	requires vsSSA != null
+	decreases *
+	requires Valid(IF(B',S1',S2'))
+{
+	// defined in thesis:
+	// merge-vars.(" if B' then S1' else S2' fi ", XLs, X, XL1i, XL2f, Y) is:
+	// " if B' then merge-vars.(S1', XLs, X, XL1i, XL2f ,Y) else merge-vars.(S2', XLs, X, XL1i, XL2f, Y) fi "
+
+	var X1 := {};
+	var B := SubstitueBooleanExpression(B', [X1], [setOf(XLi)]);
+
+	var S1 := MergeVars(S1', XLs, X, XLi, XLf, Y, vsSSA);
+	var S2 := MergeVars(S2', XLs, X, XLi, XLf, Y, vsSSA);
+
+	S := IF(B, S1, S2);
+}
+
+method DoFromSSA(B' : BooleanExpression, S' : Statement, XLs: set<Variable>, X: seq<Variable>, XLi: seq<Variable>, XLf: seq<Variable>, Y: set<Variable>, vsSSA: VariablesSSA) returns (S: Statement)
+	requires vsSSA != null
+	decreases *
+	requires Valid(DO(B',S'))
+{
+	// defined in thesis:
+	// merge-vars.(" while B' do S1' od ", XLs, X, (XL1i, XL2i), XL2i, Y) is:
+	// " while B do merge-vars.(S1', XLs, X, (XL1i, XL2i), (XL1i, XL2i), Y) od "
+
+	var XL2i := setOf(XLi) * setOf(XLf);
+	var XL1i := setOf(XLi) - XL2i;
+	var X1 := {}; // TODO
+	var X2 := {}; // TODO
+	var B := SubstitueBooleanExpression(B', [X1,X2], [XL1i,XL2i]);
+
+	S := MergeVars(S', XLs, X, XLi, XLi, Y, vsSSA);
+	S := DO(B, S);
 }
